working on the array plugin. - proving lemmas at the moment.

src/sep/Array.v
@@ -1,49 +1,126 @@
 Require Import DepList List.
 Require Import Expr SepExpr SymEval.
-Require Import SepIL SepTac.
+Require Import Word Memory IL SepIL SepTac.
+Require Import EqdepClass.
 
-Module BedrockEvaluator.
-  Module E := EvaluatorPlugin (BedrockHeap) (ST).
-  Module Import SEP := E.SEP.
+Module BedrockArrayEvaluator (P : EvaluatorPluginType BedrockHeap SepIL.ST).
+  Module Import SEP := P.SEP.
 
   Definition pcIndex : nat := 0.
   Definition stateIndex : nat := 1.
   
-  Definition addr_type :=
-    {| Impl := W
-     ; Eq := seq_dec 
+  Definition content_type :=
+    {| Expr.Impl := list W
+     ; Expr.Eq := seq_dec 
      |}.
 
-  Definition word_type :=
-    {| Impl := W
-     ; Eq := seq_dec 
-     |}.
+  Definition types := bedrock_types ++ content_type :: nil.
 
-  Definition wtypes := bedrock_types ++ addr_type :: word_type :: nil.
+  Fixpoint wbuffer (st : W) (ls : list W) : hprop (tvarD types (tvType pcIndex)) (tvarD types (tvType stateIndex)) nil :=
+    match ls with
+      | nil => emp _ _ 
+      | l :: ls =>
+        st ==> l * wbuffer (st ^+ $ 4)  ls
+    end%Sep.
 
-  Definition ptsto32_ssig : ssignature wtypes (tvType pcIndex) (tvType stateIndex).
+  Definition wbuffer_ssig : ssignature types (tvType pcIndex) (tvType stateIndex).
   refine (
-  {| SepExpr.SDomain := tvType 2 :: tvType 3 :: nil
+  {| SepExpr.SDomain := tvType 0 :: tvType 2 :: nil
    ; SepExpr.SDenotation := _
    |}).
-  refine (ptsto32 _).
+  refine (wbuffer).
   Defined.
 
-  Definition wordIndex := 3.
-  Definition ptrIndex := 2.
-  Lemma wordIndex_ptrIndex : wordIndex <> ptrIndex.
-    intro. inversion H.
-  Qed.
+  Definition wordIndex := 0.
+  Definition ptrIndex := 0.
 
-  Variable funcs : functions wtypes.
+  Variable funcs' : functions types.
+
+  Variable plusIdx : nat.
+  Variable consIdx : nat.
+  Hypothesis plusIdx_consIdx : plusIdx <> consIdx.
+
+  Definition plus_sig : signature types.
+    refine (
+  {| Expr.Domain := tvType wordIndex :: tvType wordIndex :: nil
+   ; Expr.Range := tvType wordIndex
+   ; Expr.Denotation := _
+   |}); simpl.
+    eapply wplus.
+  Defined.
+
+  Definition cons_sig : signature types.
+    refine (
+  {| Expr.Domain := tvType wordIndex :: tvType 2 :: nil
+   ; Expr.Range := tvType 2
+   ; Expr.Denotation := _
+   |}); simpl.
+    eapply cons.
+  Defined.
+
+  Definition funcs : functions types :=
+    Env.updateAt plus_sig (Env.updateAt cons_sig funcs' consIdx) plusIdx.
+
+  Fixpoint get_nth (e : expr types) (n : nat) : option (expr types) :=
+    match e with 
+      | Expr.Func i (hd :: tl :: nil) =>
+        if equiv_dec i consIdx then 
+          (* this is a cons cell *)
+          match n with
+            | 0 => Some hd
+            | S n => get_nth tl n
+          end
+        else None
+      | _ => None
+    end.
+
+  Lemma get_nth_correct : forall uvars vars e eD n x,
+    exprD funcs uvars vars e (tvType 2) = Some eD ->
+    get_nth e n = Some x ->
+    match exprD funcs uvars vars x (tvType wordIndex) with
+      | Some y => nth_error eD n = Some y
+      | None => False
+    end.
+  Proof.
+    simpl. induction e; simpl; try congruence.
+    intros. 
+    repeat match goal with
+             | [ H : context [ match ?X with
+                                 | nil => _ 
+                                 | _ :: _ => _
+                               end ] |- _ ] =>
+               (destruct X; [ try congruence | try congruence ]); [ ]
+             | [ H : context [ equiv_dec ?X ?Y ] |- _ ] =>
+               destruct (equiv_dec X Y); try congruence
+           end.
+    unfold funcs in H0.
+    erewrite Env.nth_error_updateAt_not in H0.
+    2: rewrite e1; generalize plusIdx_consIdx; eauto.
+    2: rewrite e1; eapply Env.nth_error_updateAt.
+    simpl in H0.
+    fold funcs in *.
+    destruct n;
+    repeat match goal with
+             | [ H : context [ match ?X with
+                                 | None => _ 
+                                 | Some _ => _
+                               end ] |- _ ] =>
+               revert H; case_eq X; intros; try congruence
+             | [ H : Some _ = Some _ |- _ ] => inversion H; clear H; subst
+           end.
+    rewrite H0; auto.
+    simpl.
+    inversion H; clear H. inversion H6; clear H6. subst. clear H9.
+    eapply H8; eauto.
+  Qed.
 
   (** TODO: maybe this should be like unification? 
    ** - in that case the substitution is an effect and needs to be
    **   threaded through the computation (monadically?)
    **)
-  Variable expr_equal : forall (hyps : list (expr wtypes)) (tv : tvar) (a b : expr wtypes), bool.
+  Variable expr_equal : forall (hyps : list (expr types)) (tv : tvar) (a b : expr types), bool.
   Variable expr_equal_correct : 
-    forall (hyps : list (expr wtypes)) (tv : tvar) (a b : expr wtypes),
+    forall (hyps : list (expr types)) (tv : tvar) (a b : expr types),
       expr_equal hyps tv a b = true ->
       forall uvars vars, 
         AllProvable funcs uvars vars hyps ->
@@ -51,21 +128,136 @@ Module BedrockEvaluator.
           | Some l , Some r => l = r
           | _ , _ => False
         end.
+  
+  Ltac expose :=
+    repeat (unfold wordIndex, ptrIndex in *; 
+            match goal with 
+              | [ H : match applyD _ _ ?A _ _ with
+                        | Some _ => _ 
+                        | None => False 
+                      end |- _ ] =>
+              destruct A; simpl in H; try (exfalso; assumption)
+              | [ H : context [ match exprD ?A ?B ?C ?D ?E with
+                          | None => _
+                          | Some _ => _
+                        end ] |- _ ] =>
+              generalize dependent H; case_eq (exprD A B C D E); simpl; intros; 
+                try (exfalso; assumption)
+              | [ H : context [ match expr_equal ?A ?B ?C ?D with
+                                  | true => _
+                                  | false => _
+                                end ] |- _ ] =>
+                generalize dependent H; case_eq (expr_equal A B C D); intros; 
+                  try (exfalso; congruence)
+              | [ H : expr_equal ?A ?B ?C ?D = true 
+                , H' : AllProvable _ _ _ ?A |- _ ] =>
+                generalize (@expr_equal_correct _ _ _ _ H _ _ H'); clear H; intros
+              | [ H : Some _ = Some _ |- _ ] =>
+                inversion H; clear H; subst
+              | [ H : exprD _ _ _ _ _ = Some _ |- _ ] =>
+                rewrite H in *
+            end; simpl in * ).
 
-  Definition sym_read_word_ptsto32 (hyps args : list (expr wtypes)) (p : expr wtypes) 
-    : option (expr wtypes) :=
-    match args with
-      | p' :: v' :: nil => 
-        if expr_equal hyps (tvType ptrIndex) p p' then Some v' else None
+
+  Definition divBy4 (hyps : list (expr types)) (e : expr types) : option nat :=
+    match e with
+      | Expr.Const t w => 
+        match equiv_dec (tvType 0) t with
+          | left pf =>
+            match pf in _ = t return tvarD types t -> option nat with
+              | refl_equal => fun x => None
+            end w
+          | right _ => None
+        end            
       | _ => None
     end.
-  Definition sym_write_word_ptsto32 (hyps args : list (expr wtypes)) (p v : expr wtypes)
-    : option (list (expr wtypes)) :=
+
+  Definition extractIndex (hyps : list (expr types)) (base e : expr types) : option nat := 
+    if expr_equal hyps (tvType ptrIndex) e base then 
+      Some 0
+    else 
+      match e with 
+        | Expr.Func i (l :: r :: nil) =>
+          match equiv_dec i plusIdx , expr_equal hyps (tvType ptrIndex) l base with
+            | left _ , true => divBy4 hyps r
+            | _ , _ => None
+          end
+        | _ => None
+      end.
+
+  Lemma divBy4_correct : forall uvars vars hyps e eD i,
+    divBy4 hyps e = Some i ->
+    AllProvable funcs uvars vars hyps ->
+    exprD funcs uvars vars e (tvType ptrIndex) = Some eD ->
+    eD = $ (4 * i).
+  Proof.
+    intros. destruct e; simpl in H; try congruence.
+    destruct (equiv_dec (tvType 0) t); try congruence.
+    unfold equiv in *.
+    generalize dependent t0. generalize e.
+    rewrite <- e. 
+    intro. rewrite (UIP_refl e0). congruence.
+  Qed.
+
+  Lemma extractIndex_correct : forall uvars vars hyps b bD e eD i,
+    extractIndex hyps b e = Some i ->
+    AllProvable funcs uvars vars hyps ->
+    exprD funcs uvars vars b (tvType ptrIndex) = Some bD ->
+    exprD funcs uvars vars e (tvType ptrIndex) = Some eD ->
+    eD = bD ^+ $ (4 * i).
+  Proof.
+    unfold extractIndex. intros. 
+    revert H. case_eq (expr_equal hyps (tvType ptrIndex) e b); intros.
+    inversion H3; clear H3; subst.
+    eapply expr_equal_correct in H; eauto.
+    rewrite H1 in *. rewrite H2 in *. subst. simpl in *. admit.
+    
+    destruct e; try congruence.
+    do 3 match goal with
+      | [ H : context [ match ?A with
+                          | nil => _ 
+                          | _ :: _ => _
+                        end ] |- _ ] =>
+      (destruct A; simpl in H; try congruence); [ ]
+    end.
+    clear H.
+    destruct (equiv_dec f plusIdx); try congruence.
+    rewrite e1 in *. clear e1.
+    revert H3. case_eq (expr_equal hyps (tvType ptrIndex) e b); intros; try congruence.
+
+    simpl in H2.
+    unfold funcs in H2.
+    rewrite Env.nth_error_updateAt in H2. simpl in H2.
+    fold funcs in H2.
+    eapply expr_equal_correct in H; eauto.
+    rewrite H1 in *.
+    unfold ptrIndex, wordIndex in *.
+    destruct (exprD funcs uvars vars0 e (tvType 0)); subst; try congruence.
+    revert H2.
+    case_eq (exprD funcs uvars vars0 e0 (tvType 0)); intros; try congruence.
+    inversion H2; clear H2; subst.
+    eapply divBy4_correct in H3; eauto. subst; eauto.
+  Qed.
+
+(*
+  Definition sym_read_word_wbuffer (hyps args : list (expr types)) (p : expr types) 
+    : option (expr types) :=
+    match args with
+      | p' :: v' :: nil => 
+        if expr_equal hyps (tvType ptrIndex) p p' 
+          then Some v'
+          else None
+      | _ => None
+    end.
+(*
+  Definition sym_write_word_wbuffer (hyps args : list (expr types)) (p v : expr types)
+    : option (list (expr types)) :=
     match args with
       | p' :: v' :: nil =>
         if expr_equal hyps (tvType ptrIndex) p p' then Some (p :: v :: nil) else None
       | _ => None
     end.
+*)
 
   Ltac expose :=
     repeat (unfold wordIndex, ptrIndex in *; 
@@ -96,11 +288,11 @@ Module BedrockEvaluator.
                 rewrite H in *
             end; simpl in * ).
 
-  Lemma sym_read_ptsto32_correct : forall args uvars vars cs hyps pe ve m stn,
-    sym_read_word_ptsto32 hyps args pe = Some ve ->
+  Lemma sym_read_wbuffer_correct : forall args uvars vars cs hyps pe ve m stn,
+    sym_read_word_wbuffer hyps args pe = Some ve ->
     AllProvable funcs uvars vars hyps ->
     match 
-      applyD (exprD funcs uvars vars) (SDomain ptsto32_ssig) args _ (SDenotation ptsto32_ssig)
+      applyD (exprD funcs uvars vars) (SDomain wbuffer_ssig) args _ (SDenotation wbuffer_ssig)
       with
       | None => False
       | Some p => ST.satisfies cs p stn m
@@ -112,6 +304,7 @@ Module BedrockEvaluator.
     end.
   Proof.
     simpl; intros; expose.
+    rewrite 
     unfold ST.satisfies in H3. PropXTac.propxFo.
   Qed.
 
@@ -150,25 +343,18 @@ Module BedrockEvaluator.
     eapply smem_set_get_valid_word; eauto.
   Qed.
 
-  Print E.SymEval.
+  Print P.SymEval.
   
   
 
-  Definition SymEval_ptsto32 : @E.SymEval wtypes (tvType stateIndex) (tvType pcIndex) 
+  Definition SymEval_ptsto32 : @P.SymEval types (tvType stateIndex) (tvType pcIndex) 
     (tvType ptrIndex) (tvType wordIndex)
     (fun stn => ST.HT.smem_get_word (IL.implode stn))
     (fun stn => ST.HT.smem_set_word (IL.explode stn))
     funcs ptsto32_ssig.
-  eapply E.Build_SymEval.
+  eapply P.Build_SymEval.
   eapply sym_read_ptsto32_correct.
   eapply sym_write_word_ptsto32_correct.
   Defined.  
-
-(*    {| E.sym_read_word := sym_read_word_ptsto32 : list (expr (E.wtypes wtypes ptrIndex wordIndex)) -> _
-     ; E.sym_write_word := sym_write_word_ptsto32 
-     ; E.sym_read_word_correct := sym_read_word_ptsto32_correct
-     ; E.sym_write_word_correct := sym_write_word_ptsto32_correct
-     |}.
 *)
-
-End BedrockEvaluator.
+End BedrockArrayEvaluator.
